#import "template.typ": *

= 05/02/2026: $f(x) = (arctan^5(x))/(sqrt(arccos^4(x))) + (sin^2(x))/(cot^2(x)) , " "f'(0.7) = ?$

To start with the derivative is defined and split into two separate derivatives using the *sum rule*, this is shown in *@eq-1-1*.

$
  f'(x) = d/(d x) (f(x)) = d/(d x)((arctan^5(x))/(sqrt(arccos^4(x)))) + d/(d x) ((sin^2(x))/(cot^2(x)))
$<eq-1-1>

The first section of the derivative can then be solved using a combination of the *quotient rule* and *chain rule*, the $u$ and $v$s are shown in *@eq-1-2*.

$
  "Let" u = arctan^5(x) quad v = sqrt(arccos^4(x))\
$<eq-1-2>

To differentiate $u$ and $v$, chain rule can be used. To obtain $(d u)/(d x)$ the chain rule is applied in *@eq-1-3*.

$
  u = arctan^5(x) --> "Let" z = arctan(x) therefore u = z^5\
  (d z)/(d x) = 1/(1+x^2) quad (d u)/(d z) = 5 z^4\
  (d u)/(d x) = (d u)/(d z) dot (d z)/(d x) = (5 z^4)/(1+x^2) = (5 arctan^4(x))/(1+x^2)
$<eq-1-3>

To obtain an expression for $(d v)/(d x)$ chain rule can be used twice, this is shown in *@eq-1-4*.

$
  v = sqrt(arccos^4(x)) --> "Let" z = arccos^4(x) therefore v = sqrt(z)\
  z = arccos^4(x) -->"Let" q = arccos(x) therefore z = q^4\
  (d z)/(d q) = 4 q^3 quad (d q)/(d x) = 1/(sqrt(1-x^2)) quad (d v)/(d z) = 1/(2sqrt(z))\
  (d v)/(d x) = (d v)/(d z) dot (d z)/(d x) = (d v)/(d z) dot (d z)/(d q) dot (d q)/(d x) = (4 q^3)/(2sqrt(z) (sqrt(1-x^2))) = (4 arccos^3(x))/(2 sqrt(arccos^4(x)) (sqrt(1-x^2))) = ...\
  ...= (2 arccos(x))/(sqrt(1-x^2))
$<eq-1-4>

Now that the expressions for $(d u)/(d x)$ and $(d v)/(d x)$ have been obtained, teh quotient rule can be applied to obtain $f'(x)$ for the first term, this is shown in *@eq-1-5*.

$
  "Let" u = arctan^5(x) quad v = sqrt(arccos^4(x))\
  (d u)/(d x) = (5 arctan^4(x))/(1+x^2) quad (d v)/(d x) = (2 arccos(x))/(sqrt(1-x^2))\
  A' = 1/(v^2) [(d u)/(d x) v - u (d v)/(d x)] = 1/(arccos^4(x))[ (5 arctan^4(x)arccos^2(x))/(1+x^2) + (2 arctan^5(x)arccos(x))/(sqrt(1-x^2))]
$<eq-1-5>

The second section of the expression can first be simplified using trigonometric expressions and then the quotient rule can be applied. The initial trig simplification is shown in *@eq-1-6*.

$
  B = (sin^2(x))/(cot^2(x)) = (sin^4(x))/(cos^2(x)) quad "As " cot x = (cos x)/(sin x)
$<eq-1-6>

*@eq-1-6* can be differentiated using a mixture of chain rule and quotient rule, the $u$ and $v$ are defined in *@eq-1-7*

$
  "Let" u = sin^4(x) quad v = cos^2(x)\
$<eq-1-7>

An expression for $(d u)/(d x)$ can be generated by using the chain rule shown in *@eq-1-8*.

$
  u = sin^4(x) --> "Let" z = sin(x) therefore u = z^4\
  (d z)/(d x) = cos(x) quad (d u)/(d z) = 4 z^3\
  (d u)/(d x) = (d u)/(d z) dot (d z)/(d x) = 4cos(x)z^3 = 4 cos(x)sin^3(x)
$<eq-1-8>

An expression for $(d v)/(d x)$ can be generated by using the chain rule shown in *@eq-1-9*.

$
  u = cos^2(x) --> "Let" z = cos(x) therefore u = z^2\
  (d z)/(d x) = -sin(x) quad (d u)/(d z) = 2z\
  (d u)/(d x) = (d u)/(d z) dot (d z)/(d x) = -2sin(x) z = -2sin(x)cos(x)
$<eq-1-9>

Now that an expression for $(d u)/(d x)$  and $(d v)/(d x)$ have been defined, the quotient rule can be applied, as shown in *@eq-1-10*

$
  "Let" u = sin^4(x) quad v = cos^2(x)\
  (d u)/(d x) = 4 sin^3(x)cos(x) quad (d v)/(d x) = -2sin(x)cos(x)\
  B' = 1/(v^2) [(d u)/(d x) v - u (d v)/(d x)] = 1/(cos^2(x))[4sin^3(x)cos^3(x) + 2sin^5(x)cos(x)] =...\
  ...= 4sin^3(x)cos(x) + (2sin^5(x))/cos(x)
$<eq-1-10>

Combining the $A'$ and $B'$ terms together yield a final expression for $f'(x)$ can be constructed, this is shown in *@eq-1-10*.

$
  f'(x) = 1/(arccos^4(x))[ (5 arctan^4(x)arccos^2(x))/(1+x^2) + (2 arctan^5(x)arccos(x))/(sqrt(1-x^2))] + ... \ .. + 4sin^3(x)cos(x) + (2sin^5(x))/cos(x)
$<eq-1-11>

To solve the question, $x = 0$ is substituted into $f'(0)$,  which is shown in *@eq-1-11*.

$
  f'(0) = 2.498(0.300 + 0.189) +0.818 + 0.2901 approx 2.32 " (2 d.p)"
$<eq-1-12>

#pagebreak()
